common/Separation.v
@@ -868,31 +868,25 @@ Proof.
 - eauto.
 Qed.
 
-Lemma external_call_parallel_rule:
-  forall (F V: Type) ef (ge: Genv.t F V) vargs1 m1 t vres1 m1' m2 j P vargs2,
-  external_call ef ge vargs1 m1 t vres1 m1' ->
-  m2 |= minjection j m1 ** globalenv_inject ge j ** P ->
-  Val.inject_list j vargs1 vargs2 ->
-  exists j' vres2 m2',
-     external_call ef ge vargs2 m2 t vres2 m2'
-  /\ Val.inject j' vres1 vres2
-  /\ m2' |= minjection j' m1' ** globalenv_inject ge j' ** P
-  /\ inject_incr j j'
-  /\ inject_separated j j' m1 m2.
+Lemma minjection_incr j m1 m2 j' m1' m2' P:
+  m2 |= minjection j m1 ** P ->
+  Mem.inject j' m1' m2' ->
+  Mem.unchanged_on (loc_unmapped j) m1 m1' ->
+  Mem.unchanged_on (loc_out_of_reach j m1) m2 m2' ->
+  inject_incr j j' ->
+  inject_separated j j' m1 m2 ->
+  (forall b ofs p,
+      Mem.valid_block m1 b ->
+      Mem.perm m1' b ofs Max p ->
+      Mem.perm m1 b ofs Max p) ->
+  m2' |= minjection j' m1' ** P.
 Proof.
-  intros until vargs2; intros CALL SEP ARGS.
+  intros SEP INJ' UNCH1 UNCH2 INCR ISEP MAXPERMS.
   destruct SEP as (A & B & C). simpl in A.
-  exploit external_call_mem_inject; eauto.
-  eapply globalenv_inject_preserves_globals. eapply sep_pick1; eauto.
-  intros (j' & vres2 & m2' & CALL' & RES & INJ' & UNCH1 & UNCH2 & INCR & ISEP).
-  assert (MAXPERMS: forall b ofs p,
-            Mem.valid_block m1 b -> Mem.perm m1' b ofs Max p -> Mem.perm m1 b ofs Max p).
-  { intros. eapply external_call_max_perm; eauto. }
-  exists j', vres2, m2'; intuition auto.
   split; [|split].
 - exact INJ'.
 - apply m_invar with (m0 := m2).
-+ apply globalenv_inject_incr with j m1; auto.
++ assumption.
 + eapply Mem.unchanged_on_implies; eauto.
   intros; red; intros; red; intros.
   eelim C; eauto. simpl. exists b0, delta; auto.
@@ -902,6 +896,33 @@ Proof.
   eelim C; eauto. simpl. exists b0, delta; split; auto. apply MAXPERMS; auto.
   eapply Mem.valid_block_inject_1; eauto.
 + exploit ISEP; eauto. intros (X & Y). elim Y. eapply m_valid; eauto.
+Qed.
+
+Lemma external_call_parallel_rule:
+  forall (F V: Type) ef (ge: Genv.t F V) vargs1 m1 t vres1 m1' m2 j P vargs2,
+  external_call ef ge vargs1 m1 t vres1 m1' ->
+  m2 |= minjection j m1 ** globalenv_inject ge j ** P ->
+  Val.inject_list j vargs1 vargs2 ->
+  exists j' vres2 m2',
+     external_call ef ge vargs2 m2 t vres2 m2'
+  /\ Val.inject j' vres1 vres2
+  /\ Mem.unchanged_on (loc_unmapped j) m1 m1'
+  /\ m2' |= minjection j' m1' ** globalenv_inject ge j' ** P
+  /\ inject_incr j j'
+  /\ inject_separated j j' m1 m2.
+Proof.
+  intros until vargs2; intros CALL SEP ARGS.
+  pose proof SEP as (A & B & C). simpl in A.
+  exploit external_call_mem_inject; eauto.
+  eapply globalenv_inject_preserves_globals. eapply sep_pick1; eauto.
+  intros (j' & vres2 & m2' & CALL' & RES & INJ' & UNCH1 & UNCH2 & INCR & ISEP).
+  assert (MAXPERMS: forall b ofs p,
+            Mem.valid_block m1 b -> Mem.perm m1' b ofs Max p -> Mem.perm m1 b ofs Max p).
+  { intros. eapply external_call_max_perm; eauto. }
+  exists j', vres2, m2'; intuition auto.
+  eapply minjection_incr; eauto.
+  split; [|split]; eauto.
+  apply globalenv_inject_incr with j m1; auto.
 Qed.
 
 Lemma alloc_parallel_rule_2:
